Progress in safety adequacy [coneris]

theories/coneris/adequacy.v
@@ -13,7 +13,7 @@ From clutch.prob Require Import distribution.
 Import uPred.
 
 Notation con_prob_lang_mdp := (con_lang_mdp con_prob_lang).
-
+(** Normal adequacy *)
 Section adequacy.
   Context `{!conerisGS Σ}.
   
@@ -356,3 +356,327 @@ Proof.
   intros.
   by eapply wp_pgl.
 Qed.
+
+
+(** safety *)
+Definition sch_mass_1 `{Countable sch_int_state} (sch: scheduler con_prob_lang_mdp sch_int_state) :=
+  ∀ sch_cfg, SeriesC (sch sch_cfg)=1.
+
+Section safety.
+  Context `{!conerisGS Σ}.
+  
+  Lemma safety_dbind_adv `{Countable A, Countable A'}(h : A → distr A')
+    (μ : distr A) ε (ε2 : A → R) R :
+    SeriesC μ = 1  ->
+    (exists r, forall a, 0 <= ε2(a) <= r) →
+    pgl μ R ε ->
+    (∀ a, R a -> SeriesC (h a) >= 1 - ε2 a) →
+    SeriesC (μ ≫= h) >= 1 - (ε + Expval μ ε2).
+  Proof.
+    intros H' H1 Hpgl H2.
+    rewrite dbind_mass/Expval.
+    rewrite /pgl in Hpgl.
+    setoid_rewrite <-SeriesC_scal_l.
+    rewrite -H'.
+    trans (SeriesC μ - ( prob μ (λ a : A, Datatypes.negb (bool_decide (R a))) + SeriesC (λ a : A, μ a * ε2 a))); last lra.
+    replace (SeriesC μ) with (prob μ (λ a, bool_decide (R a))+prob μ (λ a, Datatypes.negb (bool_decide (R a)))); last first.
+    { rewrite /prob. rewrite -SeriesC_plus.
+      - apply SeriesC_ext. intros. case_bool_decide; simpl; lra.
+      - apply ex_seriesC_filter_bool_pos; auto.
+      - apply ex_seriesC_filter_bool_pos; auto.
+    }
+    rewrite Rminus_plus_r_l.
+    rewrite /prob.
+    rewrite Rminus_def.
+    replace (-_) with (-1 * SeriesC (λ a, μ a * ε2 a)) by lra.
+    rewrite -SeriesC_scal_l -SeriesC_plus; [|by apply ex_seriesC_filter_bool_pos|by apply ex_seriesC_scal_l, pmf_ex_seriesC_mult_fn].
+    apply Rle_ge.
+    rewrite Rcomplements.Rminus_le_0.
+    rewrite Rminus_def.
+    replace (-_) with (-1 * SeriesC (λ x : A, (if bool_decide (R x) then μ x else 0) + -1 * (μ x * ε2 x))) by lra.
+    rewrite -SeriesC_scal_l -SeriesC_plus; last first.
+    { apply ex_seriesC_scal_l, ex_seriesC_plus; first by apply ex_seriesC_filter_bool_pos.
+      apply ex_seriesC_scal_l. by apply pmf_ex_seriesC_mult_fn.
+    }
+    { setoid_rewrite SeriesC_scal_l. apply pmf_ex_seriesC_mult_fn. naive_solver. }
+    apply SeriesC_ge_0'.
+    intros a.
+    rewrite SeriesC_scal_l.
+    case_bool_decide.
+    - trans (μ a * (1 - ε2 a) - μ a + μ a * ε2 a); first lra.
+      assert (μ a * (1 - ε2 a)<= μ a * SeriesC (h a)); last lra.
+      apply Rmult_le_compat_l; first done.
+      apply Rge_le.
+      naive_solver.
+    - apply Rplus_le_le_0_compat; first real_solver.
+      assert (0<=μ a) by done.
+      assert (0<=ε2 a) by naive_solver.
+      rewrite Rmult_plus_distr_l -Rmult_assoc.
+      replace (-1*-1) with 1 by lra.
+      rewrite Rmult_0_r Rplus_0_l Rmult_1_l.
+      real_solver.
+  Qed.
+
+  Lemma safety_dbind_adv' `{Countable A, Countable A'}(h : A → distr A')
+    (μ : distr A) ε (ε2 : A → R) n R:
+    ⌜SeriesC μ = 1 ⌝ -∗
+    ⌜exists r, forall a, 0 <= ε2(a) <= r⌝ -∗
+               ⌜pgl μ R ε⌝ -∗
+               (∀ a, ⌜R a ⌝ ={∅}=∗ |={∅}▷=>^(n)⌜SeriesC (h a) >= 1 - ε2 a⌝) -∗
+               |={∅}=> |={∅}▷=>^(n) ⌜SeriesC (μ ≫= h) >= 1 - (ε + Expval μ ε2)⌝ : iProp Σ.
+  Proof.
+    iIntros (???) "H".
+    iApply (step_fupdN_mono _ _ _ (⌜(∀ a, R a -> SeriesC (h a) >= 1 - ε2 a)⌝)).
+    { iPureIntro. intros. by eapply safety_dbind_adv. }
+    iIntros (??).
+    by iApply "H".
+  Qed.
+
+  Lemma safety_dbind' `{Countable A, Countable A'}(h : A → distr A')
+    (μ : distr A) (ε : R) n:
+    ⌜0 <= ε⌝ -∗
+    ⌜SeriesC μ = 1 ⌝ -∗
+    (∀ a, |={∅}▷=>^(n)⌜SeriesC (h a) >= 1 - ε⌝) -∗
+    |={∅}=> |={∅}▷=>^(n) ⌜SeriesC (μ ≫= h) >= 1 - ε⌝ : iProp Σ.
+  Proof.
+    iIntros (? Hmass) "H".
+    pose (ε' (a:A):= ε).
+    assert (ε=0+Expval μ ε') as K.
+    { rewrite /ε'. rewrite Expval_const; last done. rewrite Hmass. simpl. lra. }
+    rewrite {2}K.
+    iPoseProof (safety_dbind_adv' _ _ 0 ε' with "[][][][H]") as "K".
+    - done.
+    - iPureIntro. exists ε. intros. naive_solver.
+    - iPureIntro. by apply pgl_trivial.
+    - iIntros. rewrite /ε'. iApply "H".
+    - rewrite /ε'.
+      rewrite Expval_const; last done.
+      by rewrite Hmass Rmult_1_r.
+  Qed.
+
+  Lemma state_step_coupl_erasure_safety `{Countable sch_int_state} (ζ : sch_int_state) es σ ε Z n (sch: scheduler con_prob_lang_mdp sch_int_state) `{H0 : !TapeOblivious sch_int_state sch}:
+    state_step_coupl σ ε Z -∗
+    (∀ σ2 ε2, Z σ2 ε2 ={∅}=∗ |={∅}▷=>^(n)
+                               ⌜SeriesC (sch_pexec sch n (ζ, (es, σ2))) >= 1 - ε2⌝) -∗
+    |={∅}=> |={∅}▷=>^(n)
+             ⌜SeriesC (sch_pexec sch n (ζ, (es, σ))) >= 1- nonneg ε⌝.
+  Proof.
+  Admitted.
+
+  Lemma state_step_coupl_erasure_safety' `{Countable sch_int_state} (ζ : sch_int_state) e es e' σ ε Z n num (sch: scheduler con_prob_lang_mdp sch_int_state) `{!TapeOblivious sch_int_state sch}:
+    ((e::es)!!num = Some e') ->
+    to_val e = None ->
+    to_val e' = None ->
+    state_step_coupl σ ε Z -∗
+    (∀ σ2 ε2, Z σ2 ε2 ={∅}=∗ |={∅}▷=>^(S n)
+                               ⌜SeriesC (prim_step e' σ2 ≫= λ '(e3, σ3, efs), sch_pexec sch n (ζ, (<[num:=e3]> (e :: es) ++ efs, σ3))) >=1- ε2⌝) -∗
+    |={∅}=> |={∅}▷=>^(S n)
+             ⌜SeriesC (prim_step e' σ ≫= λ '(e3, σ3, efs), sch_pexec sch n (ζ, (<[num:=e3]> (e :: es) ++ efs, σ3))) >= 1- nonneg ε⌝.
+  Proof.
+  Admitted.
+  
+  Lemma wp_safety_step_fupdN `{Countable sch_int_state} (ζ : sch_int_state) (ε : nonnegreal)
+    (e : expr) es (σ : state) n φ (sch: scheduler con_prob_lang_mdp sch_int_state) `{!TapeOblivious sch_int_state sch}:
+    sch_mass_1 sch->
+    state_interp σ ∗ err_interp (ε) ∗ WP e {{ v, ⌜φ v⌝ }}  ∗ ([∗ list] e'∈ es, WP e' {{ _, True%I }})  ⊢
+    |={⊤,∅}=> |={∅}▷=>^n ⌜SeriesC (sch_pexec sch n (ζ, (e::es, σ)))  >= 1 - ε⌝.
+  Proof.
+    intros Hmass.
+    iInduction n as [|n] "IH" forall (ζ ε e es σ); iIntros "((Hσh & Hσt) & Hε & Hwp & Hwps)".
+    - iApply (fupd_mask_intro); [eauto|].
+      iIntros "_".
+      iApply step_fupdN_intro; [eauto|].
+      iPureIntro.
+      rewrite sch_pexec_O dret_mass.
+      pose proof cond_nonneg ε. simpl. lra.
+    - rewrite sch_pexec_Sn /sch_step_or_final/=.
+      case_match eqn:Hval.
+      { erewrite SeriesC_ext; last (intros; by rewrite dret_id_left').
+        iApply fupd_mask_intro; first done.
+        iIntros "Hclose".
+        do 2 iModIntro.
+        iMod "Hclose". iApply "IH".
+        iFrame.
+      }
+      rewrite /sch_step. rewrite <-dbind_assoc.
+      iApply fupd_mask_intro; first done.
+      iIntros "Hclose".
+      rewrite -fupd_idemp.
+      iApply (safety_dbind' _ _ _ (S _)); [done..|].
+      iIntros ([ζ' thid]).
+      simpl. rewrite Hval.
+      destruct ((e::es)!!thid) as [chosen_e|] eqn:Hlookup; rewrite Hlookup; last first.
+      { erewrite SeriesC_ext; last first.
+        - intros.
+          by rewrite dmap_dret dret_id_left'.
+        - do 2 iModIntro. iMod "Hclose".
+          iApply "IH". iFrame. }
+      case_match eqn:Hcheckval.
+      { erewrite SeriesC_ext; last first.
+        - intros.
+          by rewrite dmap_dret dret_id_left'.
+        - do 2 iModIntro. iMod "Hclose".
+          iApply "IH". iFrame. }
+      rewrite dmap_comp/dmap-dbind_assoc.
+      erewrite (distr_ext _ _); last first.
+      { intros x. erewrite (dbind_ext_right _ _ (λ '(_,_,_), _)); last first.
+        - intros [[??]?].
+          by rewrite dret_id_left/=.
+        - done. }
+      destruct thid as [|thid].
+      + iMod "Hclose". rewrite pgl_wp_unfold/pgl_wp_pre.
+        iMod ("Hwp" with "[$]") as "Hwp".
+        rewrite -fupd_idemp.
+        iApply (state_step_coupl_erasure_safety'  with "[$Hwp]"); try done.
+        iIntros (σ2 ε2). simpl. rewrite Hval.
+        rewrite /prog_coupl.
+        iIntros "(%R&%εa & %εb & %Hred &%Hbound & %Hineq & %Hpgl & Hlift)".
+        assert (e = chosen_e) as ?; last simplify_eq.
+        { simpl in Hlookup. by simplify_eq. }
+        iApply (step_fupdN_mono _ _ _ (⌜SeriesC
+           (prim_step chosen_e σ2 ≫= λ '(e3, σ3, efs), sch_pexec sch n (ζ', (e3 :: es ++ efs, σ3))) >=
+                                         1 - (εa + Expval (prim_step chosen_e σ2) εb)⌝)).
+        { iPureIntro. simpl in *.
+          intros. etrans; first exact.
+          apply Rle_ge.
+          apply Ropp_le_cancel.
+          rewrite !Ropp_minus_distr. by apply Rplus_le_compat_r. 
+        }
+        iApply (safety_dbind_adv' _ _ _ _ (S n) with "[][][]").
+        * iPureIntro. eapply mixin_prim_step_mass; [apply con_language_mixin|done].
+        * iPureIntro. naive_solver.
+        * done.
+        * iIntros (((e' & σ') & efs) HR).
+          iMod ("Hlift" with "[//]").
+          simpl.
+          do 3 iModIntro.
+          iApply (state_step_coupl_erasure_safety with "[$]").
+          iIntros (??) ">(?&?&?&?)". iApply "IH". iFrame.
+      + simpl in Hlookup.
+        
+  Admitted.
+  
+End safety.
+
+
+Theorem wp_safety_multi Σ `{conerisGpreS Σ} `{Countable sch_int_state} (ζ : sch_int_state) n
+  (e : expr) es (σ : state) (ε : R) (sch: scheduler con_prob_lang_mdp sch_int_state) φ `{!TapeOblivious sch_int_state sch}:
+  0 <= ε →
+  sch_mass_1 sch ->
+  (∀ `{conerisGS Σ}, ⊢ ↯ ε -∗ (WP e {{ v, ⌜φ v⌝ }} ∗ [∗ list] e'∈ es, WP e' {{ _, True%I }})) →
+  SeriesC (sch_pexec sch n (ζ, (e::es, σ)))  >= 1 - ε.
+Proof.
+  intros Hε Hmass Hwp.
+  eapply pure_soundness, (step_fupdN_soundness_no_lc _ n 0).
+  iIntros (Hinv) "_".
+  iMod (ghost_map_alloc σ.(heap)) as "[%γH [Hh _]]".
+  iMod (ghost_map_alloc σ.(tapes)) as "[%γT [Ht _]]".
+  (* Handle the trivial 1 <= ε case *)
+  destruct (decide (ε < 1)) as [Hcr|Hcr]; last first.
+  { iClear "Hh Ht".
+    iApply (fupd_mask_intro); [eauto|].
+    iIntros "_".
+    iApply step_fupdN_intro; [eauto|].
+    iApply laterN_intro; iPureIntro.
+    trans 0; [by apply Rle_ge, SeriesC_ge_0|lra].
+  }
+  set ε' := mknonnegreal _ Hε.
+  iMod (ec_alloc ε') as (?) "[??]"; [done|].
+  set (HclutchGS := HeapG Σ _ _ _ γH γT _).
+  iApply (wp_safety_step_fupdN _ ε'); first done.
+  iFrame. by iApply Hwp.
+Qed.
+
+Theorem wp_safety Σ `{conerisGpreS Σ} `{Countable sch_int_state} (ζ : sch_int_state)
+  (e : expr) (σ : state) (ε : R) n (sch: scheduler con_prob_lang_mdp sch_int_state) φ `{!TapeOblivious sch_int_state sch}:
+  0 <= ε →
+  sch_mass_1 sch ->
+  (∀ `{conerisGS Σ}, ⊢ ↯ ε -∗ WP e {{ v, ⌜φ v⌝ }}) →
+  SeriesC (sch_pexec sch n (ζ, ([e], σ)))  >= 1 - ε.
+Proof.
+  iIntros (Hε Hmass Hwp).
+  eapply wp_safety_multi; [done..|].
+  iIntros.
+  iSplitL; last done.
+  by iApply Hwp.
+Qed.
+
+
+(* Definition sch_reducible `{Countable sch_int_state} (sch: scheduler con_prob_lang_mdp sch_int_state) (ζ : sch_int_state) ρ:= *)
+(*   ∀ x, sch (ζ, ρ) x > 0 -> SeriesC (step x.2 ρ) >0. *)
+  
+(* Lemma sch_pexec_safety_relate `{Countable sch_int_state} (sch: scheduler con_prob_lang_mdp sch_int_state) (ζ : sch_int_state) ρ n: *)
+(*   sch_mass_1 sch -> *)
+(*   probp (sch_pexec sch n (ζ, ρ)) (λ '(ζ', ρ), (is_final ρ ∨ sch_reducible sch ζ' ρ)) = *)
+(*   SeriesC (sch_pexec sch (S n) (ζ, ρ)). *)
+(* Proof. *)
+(*   intros Hmass. *)
+(*   revert ζ ρ. *)
+(*   induction n; intros ζ ρ. *)
+(*   { rewrite sch_pexec_O sch_pexec_1/sch_step_or_final. *)
+(*     case_match. *)
+(*     - rewrite dret_mass. *)
+(*       rewrite probp_dret_true; first done. *)
+(*       left. *)
+(*       rewrite /is_final. naive_solver. *)
+(*     - destruct (decide (sch_reducible sch ζ ρ)). *)
+(*       + rewrite probp_dret_true; last naive_solver. *)
+(*         rewrite /sch_step. *)
+(*         rewrite dbind_mass. *)
+(*         erewrite (SeriesC_ext _ (λ a, sch (ζ, ρ) a)); first by rewrite Hmass. *)
+(*         intros [ζ' ac']. *)
+(*         destruct (pmf_pos (sch (ζ, ρ)) (ζ', ac')) as [K' | <-]; last lra. *)
+(*         rewrite dmap_mass.  *)
+(*         rewrite /sch_reducible in s. *)
+(*         unshelve epose proof s (ζ', ac') _ as H1; first lra. *)
+(*         rewrite /=/con_lang_mdp_step in H1. *)
+(*         rewrite /=/con_lang_mdp_step. *)
+(*         destruct ρ. *)
+(*         case_match. *)
+(*         { simpl in *. *)
+(*           rewrite dzero_mass in H1; lra. *)
+(*         } *)
+(*         case_match; last (rewrite dret_mass; lra). *)
+(*         case_match; first (rewrite dret_mass; lra). *)
+(*         rewrite dmap_mass. *)
+(*         erewrite mixin_prim_step_mass; [lra|apply con_language_mixin|]. *)
+(*         unshelve epose proof SeriesC_gtz_ex _ _ H1 as [? H5]; first by intros. *)
+(*         rewrite dmap_pos in H5. destruct H5 as [?[->?]]. *)
+(*         clear -H5. *)
+(*         naive_solver. *)
+(*       + rewrite probp_dret_false; last first. *)
+(*         { rewrite /is_final. intros [[??]|]; naive_solver. } *)
+(*         rewrite /sch_reducible in n. *)
+(*         symmetry. apply SeriesC_0. *)
+(*         intros [ζ' cfg]. *)
+(*         rewrite /sch_step. *)
+(*         rewrite dbind_unfold_pmf. *)
+(*         apply SeriesC_0. *)
+(*         intros [ζ'' ac']. *)
+(*         rewrite dmap_unfold_pmf/=. *)
+(*         destruct (pmf_pos (sch (ζ, ρ)) (ζ'', ac')) as [|H1]; last (rewrite -H1; lra). *)
+(*         rewrite SeriesC_0; first lra. *)
+(*         intros ρ'. *)
+(*         case_bool_decide; last lra. *)
+(*         simplify_eq. *)
+(*         destruct (pmf_pos (con_lang_mdp_step con_prob_lang ac' ρ) ρ') as [|H2]; last (rewrite -H2; lra). *)
+(*         exfalso. *)
+(*         apply n. *)
+        
+(*   }  *)
+(* Admitted. *)
+
+(* Corollary wp_safety' Σ `{conerisGpreS Σ} `{Countable sch_int_state} (ζ : sch_int_state) *)
+(*   (e : expr) (σ : state) (ε : R) n (sch: scheduler con_prob_lang_mdp sch_int_state) φ `{!TapeOblivious sch_int_state sch}: *)
+(*   0 <= ε → *)
+(*   sch_mass_1 sch -> *)
+(*   (∀ `{conerisGS Σ}, ⊢ ↯ ε -∗ WP e {{ v, ⌜φ v⌝ }}) → *)
+(*   probp (sch_pexec sch n (ζ, ([e], σ))) *)
+(*     (λ '(ζ', ρ), is_final ρ \/ *)
+(*                    sch_reducible sch ζ' ρ *)
+(*     ) >= 1 - ε. *)
+(* Proof. *)
+(*   intros Hε Hmass Hwp. *)
+(*   rewrite sch_pexec_safety_relate. *)
+(*   by eapply wp_safety. *)
+(* Qed. *)
